theories/Environment/ReaderStock.v
@@ -7,11 +7,11 @@ Import ResourceNotations TermNotations REnvironmentNotations CellNotations
 
 (** * Environment - Virtual Resource Environment - Reader
 
-  In the functional transition there are two kind of environment: the resource environment and the stock. The former, defined in [REnvironment.v], represents the local memory during an instant. The latter, defined in [Stock.v], keeps local resource names with their initial value. [ReadStock] is a part of the stock. It maps resource names with terms, i.e, it binds local resource names, used for a reading interaction, with their initial value.
+  In the functional transition there are two kind of environment: the resource environment and the stock. The former, defined in [REnvironment.v], represents the local memory during an instant. The latter, defined in [Stock.v], keeps local resource names with their initial value. [ReaderStock] is a part of the storage. It maps resource names with terms, i.e, it binds local resource names, used for a reading interaction, with their initial value.
 *)
 
 (** ** Module - Virtual Resource Environment - Reader *)
-Module ReadStock <: IsLvlET.
+Module ReaderStock <: IsLvlET.
 
 Include OverlayMap Term.
 Import Raw Ext.
@@ -25,9 +25,9 @@ Module RE := REnvironment.
 
   For each instant, local resource names that represent a reading interaction have their memory cells initialized as unused with a certain term. This function takes a reader environment [rs] and an environement [V] and produces an environment where all resource names in [rs] are initialized.
 *)
-Definition init_read_func (r : resource) (v : Λ) (V : 𝐕) := (⌈ r ⤆ ⩽ v … ⩾ ⌉ V)%re.
+Definition init_readers_func (r : resource) (v : Λ) (V : 𝐕) := (⌈ r ⤆ ⩽ v … ⩾ ⌉ V)%re.
 
-Definition init_read (rs : t) (V : 𝐕) := fold init_read_func rs V.
+Definition init_readers (rs : t) (V : 𝐕) := fold init_readers_func rs V.
 
 (** **** Halts 
 
@@ -61,7 +61,7 @@ Proof.
   - reflexivity.
   - intros k' k Heqk d' d Heqd c c' Heqc; subst; now rewrite Heqc.
   - apply diamond_add.
-  - unfold ReadStock.Add; reflexivity.
+  - unfold ReaderStock.Add; reflexivity.
 Qed.
 
 Lemma valid_extend_spec (k : lvl) (rs rs' : t) :
@@ -69,110 +69,110 @@ Lemma valid_extend_spec (k : lvl) (rs rs' : t) :
 Proof.
   revert rs; induction rs' using map_induction; intros rs Hvrs Hvrs'.
   - rewrite extend_Empty_right_spec; auto.
-  - unfold ReadStock.Add in H0; rewrite H0 in *; clear H0.
+  - unfold ReaderStock.Add in H0; rewrite H0 in *; clear H0.
     rewrite extend_add_right_spec; auto.
     apply valid_add_notin_spec in Hvrs' as [Hvx [Hve Hvrs'1]]; auto.
     apply valid_add_spec; auto.
 Qed.
 
 
-(** **** [init_read] property *)
+(** **** [init_readers] property *)
 
-#[export] Instance init_read_func_proper :
- Proper (Logic.eq ==> Logic.eq ==> RE.eq ==> RE.eq) init_read_func.
+#[export] Instance init_readers_func_proper :
+ Proper (Logic.eq ==> Logic.eq ==> RE.eq ==> RE.eq) init_readers_func.
 Proof.
-  intros k' k Heqk d' d Heqd V V' HeqV; subst; unfold init_read_func.
+  intros k' k Heqk d' d Heqd V V' HeqV; subst; unfold init_readers_func.
   now rewrite HeqV.
 Qed.
 
-Lemma init_read_func_diamond : Diamond RE.eq init_read_func.
+Lemma init_readers_func_diamond : Diamond RE.eq init_readers_func.
 Proof.
-  unfold init_read_func; intros k k' d d' rs rs1 rs' Hneq Heq Heq'.
+  unfold init_readers_func; intros k k' d d' rs rs1 rs' Hneq Heq Heq'.
   rewrite <- Heq; rewrite <- Heq'.
   now rewrite RE.add_add_2; auto.
 Qed.
 
-#[local] Hint Resolve init_read_func_proper init_read_func_diamond RE.Equal_equiv : core.
+#[local] Hint Resolve init_readers_func_proper init_readers_func_diamond RE.Equal_equiv : core.
 
-Lemma init_read_Empty_spec (rs : t) (V : 𝐕) :
-  Empty rs -> RE.eq (init_read rs V) V.
+Lemma init_readers_Empty_spec (rs : t) (V : 𝐕) :
+  Empty rs -> RE.eq (init_readers rs V) V.
 Proof.
-  intro Hemp; unfold init_read.
+  intro Hemp; unfold init_readers.
   rewrite fold_Empty with (eqA := RE.eq); now auto.
 Qed.
 
-Lemma init_read_add_spec (r : resource) (v : Λ) (rs : t) (V : 𝐕) :
+Lemma init_readers_add_spec (r : resource) (v : Λ) (rs : t) (V : 𝐕) :
   ~ (In r rs) ->
-  RE.eq (init_read (add r v rs) V) (⌈ r ⤆ (⩽ v … ⩾)⌉ (init_read rs V))%re. 
+  RE.eq (init_readers (add r v rs) V) (⌈ r ⤆ (⩽ v … ⩾)⌉ (init_readers rs V))%re. 
 Proof.
-  unfold init_read; intro HnIn.
+  unfold init_readers; intro HnIn.
   rewrite fold_Add with (eqA := RE.eq); eauto.
-  - unfold init_read_func at 1; reflexivity.
+  - unfold init_readers_func at 1; reflexivity.
   - red; reflexivity.
 Qed.
 
-#[export] Instance init_read_proper : Proper (eq ==> RE.eq ==> RE.eq) init_read.
+#[export] Instance init_readers_proper : Proper (eq ==> RE.eq ==> RE.eq) init_readers.
 Proof.
-  intros rs rs' Heqrs V V' HeqV; unfold init_read.
+  intros rs rs' Heqrs V V' HeqV; unfold init_readers.
   eapply fold_Proper with (eqA := RE.eq); now eauto.
 Qed.  
 
-Lemma init_read_find_spec (rs : t) (V : 𝐕) (r : resource) (v : 𝑣) :
-  ((init_read rs V)⌊r⌋)%re = Some v -> In r rs \/ V⌊r⌋%re = Some v.
+Lemma init_readers_find_spec (rs : t) (V : 𝐕) (r : resource) (v : 𝑣) :
+  ((init_readers rs V)⌊r⌋)%re = Some v -> In r rs \/ V⌊r⌋%re = Some v.
 Proof.
   revert r v; induction rs using map_induction; intros r v Hfi.
-  - rewrite init_read_Empty_spec in Hfi; auto.
-  - unfold ReadStock.Add in H0; rewrite H0 in *; clear H0.
-    rewrite init_read_add_spec in Hfi; auto.
+  - rewrite init_readers_Empty_spec in Hfi; auto.
+  - unfold ReaderStock.Add in H0; rewrite H0 in *; clear H0.
+    rewrite init_readers_add_spec in Hfi; auto.
     rewrite RE.add_o in Hfi; destruct (Resource.eq_dec x r) as [| Hneq]; subst.
     -- now rewrite add_in_iff; repeat left.
     -- rewrite add_in_iff.
        apply IHrs1 in Hfi as [HIn | Hfi]; auto.
 Qed. 
 
-Lemma init_read_in_iff  (rs : t) (V : 𝐕) (r : resource) :
-  (r ∈ (init_read rs V))%re <-> In r rs \/ (r ∈ V)%re.
+Lemma init_readers_in_iff  (rs : t) (V : 𝐕) (r : resource) :
+  (r ∈ (init_readers rs V))%re <-> In r rs \/ (r ∈ V)%re.
 Proof.
   revert r; induction rs using map_induction; intro r; split.
-  - rewrite init_read_Empty_spec; auto.
+  - rewrite init_readers_Empty_spec; auto.
   - intros [HIn | HIn].
     -- destruct HIn as [v HM].
        exfalso; now apply (H r v).
-    -- rewrite init_read_Empty_spec; auto.
+    -- rewrite init_readers_Empty_spec; auto.
   - intro HIn.
-    unfold ReadStock.Add in H0; rewrite H0 in *; clear H0.
-    rewrite init_read_add_spec in HIn; auto.
+    unfold ReaderStock.Add in H0; rewrite H0 in *; clear H0.
+    rewrite init_readers_add_spec in HIn; auto.
     rewrite add_in_iff.
     apply RE.add_in_iff in HIn as [| HIn]; subst; auto.
     apply IHrs1 in HIn as [HIn | HIn]; auto.
-  - unfold ReadStock.Add in H0; rewrite H0 in *; clear H0.
+  - unfold ReaderStock.Add in H0; rewrite H0 in *; clear H0.
     rewrite add_in_iff.
-    rewrite init_read_add_spec; auto.
+    rewrite init_readers_add_spec; auto.
     rewrite RE.add_in_iff.
     intros [[Heq | HIn] | HIn]; subst; auto; 
     right; rewrite IHrs1; auto.
 Qed. 
 
-Lemma init_read_unused (rs : t) (V : 𝐕) (r : resource) :
-  In r rs -> REnvironment.unused r (init_read rs V).
+Lemma init_readers_unused (rs : t) (V : 𝐕) (r : resource) :
+  In r rs -> REnvironment.unused r (init_readers rs V).
 Proof.
   revert r; induction rs using map_induction; intros r HIn.
   - exfalso; destruct HIn as [v HM]; now apply (H r v).
-  - unfold ReadStock.Add in H0; rewrite H0 in *; clear H0.
-    rewrite init_read_add_spec; auto; 
+  - unfold ReaderStock.Add in H0; rewrite H0 in *; clear H0.
+    rewrite init_readers_add_spec; auto; 
     apply add_in_iff in HIn as [| HIn]; subst.
     -- apply RE.unused_add_eq_spec; now red.
     -- assert (Hneq : r <> x) by (intro; subst; contradiction).
        apply RE.unused_add_neq_spec; auto.
 Qed.
 
-(* Lemma init_read_Forall_unused : forall rsk V,
+(* Lemma init_readers_Forall_unused : forall rsk V,
   REnvironment.For_all (fun _ v => Cell.unused v) V ->
-  REnvironment.For_all (fun _ v => Cell.unused v) (init_read rsk V).
+  REnvironment.For_all (fun _ v => Cell.unused v) (init_readers rsk V).
 Proof.
   unfold REnvironment.For_all in *; intros.
-  apply init_read_find_spec in H0 as H0'; destruct H0'; auto.
-  - eapply init_read_unused in H1; eauto.
+  apply init_readers_find_spec in H0 as H0'; destruct H0'; auto.
+  - eapply init_readers_unused in H1; eauto.
     destruct H1; rewrite H0 in H1; inversion H1. now simpl.
   - eapply H; eauto.
 Qed. *)
@@ -226,82 +226,82 @@ Proof.
   apply halts_weakening; auto; lia.
 Qed.
 
-Lemma halts_init_read (k : lvl) (rs : t) (V : 𝐕) :
-  halts k rs -> RE.halts k V -> RE.halts k (init_read rs V).
+Lemma halts_init_readers (k : lvl) (rs : t) (V : 𝐕) :
+  halts k rs -> RE.halts k V -> RE.halts k (init_readers rs V).
 Proof.
   induction rs using map_induction; intros Hltrs HltV.
-  - now rewrite init_read_Empty_spec.
-  - unfold ReadStock.Add in H0; rewrite H0 in *; clear H0.
-    rewrite init_read_add_spec; auto.
+  - now rewrite init_readers_Empty_spec.
+  - unfold ReaderStock.Add in H0; rewrite H0 in *; clear H0.
+    rewrite init_readers_add_spec; auto.
     apply RE.halts_add_spec; simpl.
     apply halts_add_iff in Hltrs as [Hkte Htlrs1]; auto. 
 Qed.
 
 (** **** Morphism *)
 
-#[export] Instance in_readstock : Proper (Logic.eq ==> eq ==> iff) In.
+#[export] Instance in_ReaderStock : Proper (Logic.eq ==> eq ==> iff) In.
 Proof. intros k' k Heqk rs rs' Heqrs; subst; now rewrite Heqrs. Qed.
 
-#[export] Instance Add_readstock : 
-  Proper (Resource.eq ==> Term.eq ==> eq ==> eq ==> iff) (@ReadStock.Add Term.t).
+#[export] Instance Add_ReaderStock : 
+  Proper (Resource.eq ==> Term.eq ==> eq ==> eq ==> iff) (@ReaderStock.Add Term.t).
 Proof.
-  intros k' k Heqk d d' Heqd rs rs' Heqrs rs1 rs1' Heqrs1; unfold ReadStock.Add.
+  intros k' k Heqk d d' Heqd rs rs' Heqrs rs1 rs1' Heqrs1; unfold ReaderStock.Add.
   now rewrite Heqk, Heqd, Heqrs, Heqrs1. 
 Qed.
 
-#[export] Instance halts_readstock : Proper (Logic.eq ==> eq ==> iff) halts. 
+#[export] Instance halts_ReaderStock : Proper (Logic.eq ==> eq ==> iff) halts. 
 Proof. unfold halts; intros m n Heqm rs rs' Heqrs; subst; now rewrite Heqrs. Qed.
 
-End ReadStock.
+End ReaderStock.
 
 (** ---- *)
 
 (** ** Notation - Virtual Resource Environment - Reader *)
 
-Module ReadStockNotations.
+Module ReaderStockNotations.
 
 (** *** Scope *)
 Declare Scope rstock_scope.
 Delimit Scope rstock_scope with rk.
 
 (** *** Notation *)
-Definition 𝐖ᵣ := ReadStock.t.
+Definition 𝐖ᵣ := ReaderStock.t.
 
-Notation "V '⁺'" := (ReadStock.Ext.new_key V) (at level 16) : rstock_scope.
-Notation "∅" := ReadStock.Raw.empty (at level 0, no associativity) : rstock_scope. 
-Notation "r '∉' Re" := (~ (ReadStock.Raw.In r Re)) (at level 75, no associativity) : rstock_scope. 
-Notation "'isEmpty(' Re ')'" := (ReadStock.Empty Re) (at level 20, no associativity) : rstock_scope. 
-Notation "'Add'" := (ReadStock.Add) (at level 20, no associativity) : rstock_scope. 
-Notation "R '⌊' x '⌋'"  := (ReadStock.Raw.find x R) (at level 15, x constr) : rstock_scope.
-Notation "'max(' R ')'"  := (ReadStock.Ext.max_key R) (at level 15) : rstock_scope.
-Notation "⌈ x ⤆ v '⌉' R" := (ReadStock.Raw.add x v R) 
+Notation "V '⁺'" := (ReaderStock.Ext.new_key V) (at level 16) : rstock_scope.
+Notation "∅" := ReaderStock.Raw.empty (at level 0, no associativity) : rstock_scope. 
+Notation "r '∉' Re" := (~ (ReaderStock.Raw.In r Re)) (at level 75, no associativity) : rstock_scope. 
+Notation "'isEmpty(' Re ')'" := (ReaderStock.Empty Re) (at level 20, no associativity) : rstock_scope. 
+Notation "'Add'" := (ReaderStock.Add) (at level 20, no associativity) : rstock_scope. 
+Notation "R '⌊' x '⌋'"  := (ReaderStock.Raw.find x R) (at level 15, x constr) : rstock_scope.
+Notation "'max(' R ')'"  := (ReaderStock.Ext.max_key R) (at level 15) : rstock_scope.
+Notation "⌈ x ⤆ v '⌉' R" := (ReaderStock.Raw.add x v R) 
                              (at level 15, x constr, v constr) : rstock_scope.
-Notation "'[⧐' lb '–' k ']' t" := (ReadStock.shift lb k t) 
+Notation "'[⧐' lb '–' k ']' t" := (ReaderStock.shift lb k t) 
                                    (at level 65, right associativity) : rstock_scope.
 
-Infix "⊆" := ReadStock.Submap (at level 60, no associativity) : rstock_scope. 
-Infix "∈" := ReadStock.Raw.In (at level 60, no associativity) : rstock_scope. 
-Infix "=" := ReadStock.eq : rstock_scope.
-Infix "∪" := ReadStock.extend : rstock_scope.
-Infix "⊩" := ReadStock.valid (at level 20, no associativity) : rstock_scope.
+Infix "⊆" := ReaderStock.Submap (at level 60, no associativity) : rstock_scope. 
+Infix "∈" := ReaderStock.Raw.In (at level 60, no associativity) : rstock_scope. 
+Infix "=" := ReaderStock.eq : rstock_scope.
+Infix "∪" := ReaderStock.extend : rstock_scope.
+Infix "⊩" := ReaderStock.valid (at level 20, no associativity) : rstock_scope.
 
 (** *** Morphism *)
 
-Import ReadStock.
+Import ReaderStock.
 
 #[export] Instance max_rk : Proper (eq ==> Logic.eq) (Ext.max_key) := Ext.max_key_eq.
 #[export] Instance new_rk : Proper (eq ==> Logic.eq) (Ext.new_key) := Ext.new_key_eq.
-#[export] Instance in_rk : Proper (Logic.eq ==> ReadStock.eq ==> iff) (ReadStock.Raw.In) := _.
+#[export] Instance in_rk : Proper (Logic.eq ==> ReaderStock.eq ==> iff) (ReaderStock.Raw.In) := _.
 #[export] Instance find_rk : Proper (Logic.eq ==> eq ==> Logic.eq) (Raw.find) := _.
-#[export] Instance Empty_rk : Proper (ReadStock.eq ==> iff) (ReadStock.Empty) := _.
+#[export] Instance Empty_rk : Proper (ReaderStock.eq ==> iff) (ReaderStock.Empty) := _.
 #[export] Instance Add_rk : 
-  Proper (Resource.eq ==> Term.eq ==> eq ==> eq ==> iff) (@ReadStock.Add Term.t) := _.
+  Proper (Resource.eq ==> Term.eq ==> eq ==> eq ==> iff) (@ReaderStock.Add Term.t) := _.
 #[export] Instance add_rk : 
   Proper (Resource.eq ==> Term.eq ==> eq ==> eq) (@Raw.add Term.t) := _.
 #[export] Instance Submap_rk : Proper (eq ==> eq ==> iff) Submap := _.
-#[export] Instance Submap_rk_po : PreOrder ReadStock.Submap := Submap_po.
-#[export] Instance valid_rk : Proper (Logic.eq ==> ReadStock.eq ==> iff) ReadStock.valid := _.
+#[export] Instance Submap_rk_po : PreOrder ReaderStock.Submap := Submap_po.
+#[export] Instance valid_rk : Proper (Logic.eq ==> ReaderStock.eq ==> iff) ReaderStock.valid := _.
 #[export] Instance shift_rk : Proper (Logic.eq ==> Logic.eq ==> eq ==> eq) shift := _.
-#[export] Instance halts_rk: Proper (Logic.eq ==> ReadStock.eq ==> iff) ReadStock.halts := _.
+#[export] Instance halts_rk: Proper (Logic.eq ==> ReaderStock.eq ==> iff) ReaderStock.halts := _.
 
-End ReadStockNotations.
+End ReaderStockNotations.
